Remove handle.
We drastically simplify the model by removing `handle`.
We shall next defunctionalize `Fitree`, hard-coding SSA
effects into our `Fitree`. This means that we will not
need to reason about `Vis` in general, but only in particular
about `Read, Write` (from `SSAEnvE`), plus `UB` from `UBE`.

We will retain a notion of extensibility of semantics, because
we will describe how to graft together different handlers for
operations. This will be the work of our `Semantics S` typeclass,
which will have instances for sums of dialects (`d1 + d2`).

MLIR/Semantics/UB.lean
@@ -20,16 +20,19 @@ abbrev UBT := ExceptT String
 
 inductive UBE: Type → Type :=
   | UB {α: Type} [Inhabited α]: Option String → UBE α
+  | Unhandled {α: Type} [Inhabited α]: UBE α
 
 @[simp_itree]
 def UBE.handle {E}: UBE ~> UBT (Fitree E) := fun _ e =>
   match e with
+  | Unhandled => throw "<unhandled>"
   | UB none => throw "<UB>"
   | UB (some msg) => throw s!"<UB: {msg}>"
 
 @[simp_itree]
 def UBE.handle! {E}: UBE ~> Fitree E := fun _ e =>
   match e with
+  | Unhandled => panic! "<unhandled>"
   | UB none => panic! "<UB>"
   | UB (some msg) => panic! s!"<UB: {msg}>"
 
